finished most of the merge sort proofs; this left some bug in the OCaml code...?

examples/MergeSort.v
@@ -7,9 +7,21 @@ Import ListNotations.
 Require Import Coq.Arith.Peano_dec.
 Require Import Coq.Arith.Compare_dec.
 Require Import Coq.Arith.Le.
+Require Import Coq.Arith.Lt.
 Require Import Coq.Arith.Plus.
+Require Import Coq.Arith.Minus.
 Require Import Coq.Arith.Div2.
+Require Import Coq.Wellfounded.Wellfounded.
+Require Import Coq.Relations.Relation_Operators.
+Require Import Coq.Arith.Wf_nat.
 
+
+(***
+ *** Definitions of "sorted" and "permutation-of"
+ ***)
+
+(* A list is sorted iff it is empty, a singleton, or its first element is no
+greater than its second and its tail is sorted. *)
 Fixpoint sorted (l: list nat) : Prop :=
   match l with
     | [] => True
@@ -20,9 +32,124 @@ Fixpoint sorted (l: list nat) : Prop :=
        end)
   end.
 
+(* Two lists are permutations of each other iff they have the same number of
+occurrences of all elements. *)
 Definition permOf (l1 l2: list nat) : Prop :=
   forall x, count_occ eq_nat_dec l1 x = count_occ eq_nat_dec l2 x.
 
+Lemma permOf_refl l : permOf l l.
+  intro x; reflexivity.
+Qed.
+
+Lemma permOf_sym l1 l2 : permOf l1 l2 -> permOf l2 l1.
+  intros pof x; symmetry; apply (pof x).
+Qed.
+
+Lemma permOf_trans l1 l2 l3 :
+  permOf l1 l2 -> permOf l2 l3 -> permOf l1 l3.
+  intros pof12 pof23 x.
+  rewrite (pof12 x). apply pof23.
+Qed.
+
+Lemma permOf_cons x l1 l2 :
+  permOf l1 l2 -> permOf (x::l1) (x::l2).
+  intros pof y. destruct (eq_nat_dec x y).
+  rewrite (count_occ_cons_eq _ _ e); rewrite (count_occ_cons_eq _ _ e).
+  f_equal; apply pof.
+  rewrite (count_occ_cons_neq _ _ n); rewrite (count_occ_cons_neq _ _ n).
+  apply pof.
+Qed.
+
+Lemma permOf_swap x y l : permOf (x::y::l) (y::x::l).
+  intro z; unfold count_occ; fold (count_occ eq_nat_dec l).
+  destruct (eq_nat_dec x z); destruct (eq_nat_dec y z); reflexivity.
+Qed.
+
+Lemma permOf_nil_cons x l : ~(permOf [] (x::l)).
+  intro pof.
+  assert (0 = count_occ eq_nat_dec (x::l) x); [ apply pof | ].
+  rewrite (count_occ_cons_eq eq_nat_dec l eq_refl) in H.
+  discriminate.
+Qed.
+
+Lemma permOf_app_cons l1 x l2 :
+  permOf (l1 ++ x::l2) (x::l1 ++ l2).
+  induction l1.
+  intro y; reflexivity.
+  intro y.
+  unfold app; fold (app l1).
+  unfold count_occ; fold (count_occ eq_nat_dec (l1++x::l2));
+  fold (count_occ eq_nat_dec (l1++l2)).
+  rewrite (IHl1 y).
+  case_eq (eq_nat_dec a y); intros; case_eq (eq_nat_dec x y); intros.
+  unfold count_occ; rewrite H0; reflexivity.
+  unfold count_occ; rewrite H0; reflexivity.
+  unfold count_occ; rewrite H0; reflexivity.
+  unfold count_occ; rewrite H0; reflexivity.
+Qed.
+
+
+Lemma permOf_cons_in x l1 l2 :
+  permOf (x::l1) l2 -> In x l2.
+  intro pof.
+  apply (proj2 (count_occ_In eq_nat_dec _ _)).
+  rewrite <- pof.
+  unfold count_occ; destruct (eq_nat_dec x x).
+  apply lt_0_Sn.
+  elimtype False; apply (n eq_refl).
+Qed.
+
+Lemma in_split_set x l :
+  In x l -> { l1 : list nat & { l2 : list nat & l = l1 ++ x :: l2 } }.
+  induction l; intros.
+  elimtype False; apply H.
+  destruct (eq_nat_dec a x).
+  rewrite e. exists []; exists l; reflexivity.
+  assert (In x l).
+  destruct H; [ contradiction | assumption ].
+  destruct (IHl H0) as [ l1 X ]; destruct X as [ l2 e ].
+  exists (a::l1); exists l2. rewrite e. reflexivity.
+Qed.
+
+Lemma permOf_cons_inv x l1 l2 :
+  permOf (x::l1) (x::l2) -> permOf l1 l2.
+  intros pof y.
+  assert (count_occ eq_nat_dec (x::l1) y =
+          count_occ eq_nat_dec (x::l2) y); [ apply pof | ].
+  unfold count_occ in H; fold (count_occ eq_nat_dec) in H.
+  destruct (eq_nat_dec x y).
+  injection H; intros; assumption.
+  assumption.
+Qed.
+
+Lemma permOf_app l1 l1' l2 l2' :
+  permOf l1 l1' -> permOf l2 l2' -> permOf (l1++l2) (l1'++l2').
+  revert l1' l2 l2'; induction l1; intros.
+  destruct l1'.
+  assumption.
+  elimtype False; apply (permOf_nil_cons n l1'); assumption.
+  assert (In a l1').
+  apply (permOf_cons_in _ l1); assumption.
+  destruct (in_split_set a l1' H1) as [ l1'' X ]; destruct X as [ l2'' e ].
+  rewrite e. rewrite <- app_assoc.
+  rewrite <- app_comm_cons. rewrite <- app_comm_cons.
+  apply (permOf_trans _ (a :: l1'' ++ l2'' ++ l2')).
+  apply permOf_cons.
+  rewrite app_assoc.
+  apply IHl1.
+  rewrite e in H.
+  apply (permOf_cons_inv a).
+  apply (permOf_trans _ _ _ H).
+  apply permOf_app_cons.
+  assumption.
+  apply permOf_sym.
+  apply permOf_app_cons.
+Qed.
+
+
+(***
+ *** The high-level spec for sorting
+ ***)
 
 Spec Sorting.
 
@@ -32,6 +159,11 @@ Spec Axiom sort_correct :
 
 Spec End Sorting.
 
+
+(***
+ *** The MergeSort0 spec, which instantiates all the elements of the
+ *** DivideAndConquer_base spec for merge-sort.
+ ***)
 
 Spec MergeSort0.
 
@@ -47,80 +179,128 @@ Spec Definition IO : (D -> R -> Prop) :=
 Spec Definition smaller : (D -> D -> Prop) :=
   (fun l1 l2 => length l1 < length l2).
 
-(* The helper operations *)
-Spec Definition primitive : (D -> bool) :=
-  (fun l => if lt_dec (length l) 2 then true else false).
+(* Proof that smaller is well-founded. Note that we make this a Definition
+instead of a Theorem because DivideAndConquer_base requires well-foundedness to
+be a subtype predicate and not an axiom. *)
+Spec Definition smaller_wf : (well_founded smaller) :=
+  (well_founded_ltof _ _).
 
-(* Split l into (l1,l2) where l1 has length n *)
-Program Fixpoint list_split n (l : {l:list nat | n <= length l}) : list nat * list nat :=
+
+(***
+ *** The base case, which is directly sorting a singleton list
+ ***)
+
+(* Test if a list is empty or a singleton; leb is the decision procedure for
+deciding less-than-or-equal. *)
+Spec Definition primitive : (D -> bool) :=
+  (fun l => leb (length l) 1).
+
+(* Sorting for an empty or singleton list is just the identity *)
+Spec Definition direct_solve : (D -> R) := (fun l => l).
+
+
+(***
+ *** The decompose operation; requires list prefix and suffix
+ ***)
+
+(* Take the prefix of l of length <= n *)
+Fixpoint list_prefix n l : list nat :=
   match n with
-    | 0 => ([], l)
+    | 0 => []
     | S n' =>
       match l with
-        | [] => match (_:False) with end
-        | x::l' =>
-          let (l1,l2) := list_split n' l' in (x::l1, l2)
+        | [] => []
+        | x::l' => x :: list_prefix n' l'
       end
   end.
-Next Obligation.
-apply (le_Sn_0 _ H).
-Defined.
-Next Obligation.
-apply le_S_n; assumption.
-Defined.
 
-Theorem list_split_app n l l_pf :
-  fst (list_split n (exist _ l l_pf)) ++ snd (list_split n (exist _ l l_pf)) = l.
-  transitivity (let (l1,l2) := list_split n (exist _ l l_pf) in l1 ++ l2).
-  destruct (list_split
-              n
-              (exist (fun l0 : list nat => n <= Datatypes.length l0) l l_pf));
-    reflexivity.
-  revert l l_pf; induction n; intros.
-  unfold list_split; reflexivity.
+(* Lemma: the length of list_prefix n l is no greater than n *)
+Lemma list_prefix_len n l : length (list_prefix n l) <= n.
+  revert l; induction n; intros.
+  reflexivity.
   destruct l.
-  elimtype False; apply (le_Sn_0 _ l_pf).
-  unfold list_split; fold list_split; unfold proj1_sig.
-  replace (n0 :: l) with
-  (n0::(let (l1,l2) :=
-            (list_split
-               n
-               (exist
-                  _ l
-                  (list_split_obligation_2
-                        (S n)
-                        (exist (fun l0 : list nat => S n <= Datatypes.length l0)
-                               (n0 :: l) l_pf) n eq_refl n0 l eq_refl)))
-        in (l1 ++ l2))).
-  destruct (list_split n
-                       (exist (fun l0 : list nat => n <= Datatypes.length l0) l
-                              (list_split_obligation_2 (S n)
-                                                       (exist (fun l0 : list nat => S n <= Datatypes.length l0)
-                                                              (n0 :: l) l_pf) n eq_refl n0 l eq_refl))).
-  reflexivity.
-  f_equal.
-  rewrite IHn.
-  reflexivity.
+  apply le_0_n.
+  apply le_n_S. apply IHn.
 Qed.
 
-Program Definition list_split_len l : list nat * list nat :=
-  list_split (div2 (length l)) l.
-Next Obligation.
-admit. (* FIXME: prove this! *)
-Defined.
+(* Take the suffix of l, removing the first n elements, if they exist *)
+Fixpoint list_suffix n l : list nat :=
+  match n with
+    | 0 => l
+    | S n' =>
+      match l with
+        | [] => []
+        | x::l' => list_suffix n' l'
+      end
+  end.
 
-Spec Definition decompose : (D -> D * D) := list_split_len.
+(* Lemma: the length of list_suffix n l is length l - n *)
+Lemma list_suffix_len n l : length (list_suffix n l) = length l - n.
+  revert l; induction n; intro l; destruct l; try reflexivity.
+  unfold list_suffix; fold list_suffix.
+  unfold length; fold (length l); fold (length (list_suffix n l)).
+  apply IHn.
+Qed.
 
-Definition list_pair_smaller (l_pair1: list nat * list nat)
-           (l_pair2: list nat * list nat) : Prop :=
-  length (fst l_pair1) + length (snd l_pair1)
-  <
-  length (fst l_pair2) + length (snd l_pair2).
+(* Appending the prefix and the suffix yields the original list *)
+Lemma list_prefix_suffix_eq n l : list_prefix n l ++ list_suffix n l = l.
+  revert l; induction n; intro l; [ | destruct l ].
+  reflexivity.
+  reflexivity.
+  unfold list_prefix; fold list_prefix.
+  unfold list_suffix; fold list_suffix.
+  unfold app; fold (app (list_prefix n l)).
+  f_equal.
+  apply IHn.
+Qed.
 
-Theorem list_pair_smaller_wf : well_founded list_pair_smaller.
-admit.
-Defined.
+(* The decompose operator splits a list into prefix and suffix *)
+Spec Definition decompose : (D -> D * D) :=
+  (fun l => (list_prefix (div2 (length l)) l,
+             list_suffix (div2 (length l)) l)).
 
+(* Proof that decompose yields smaller lists. As with smaller_wf, we make this a
+Definition and not a Theorem because DivideAndConquer_base needs it as a proof
+of a subtype predicate. *)
+Definition decompose_smallerH l :
+  primitive l = false ->
+  smaller (fst (decompose l)) l /\ smaller (snd (decompose l)) l.
+  intro H; unfold decompose, smaller, def, fst, snd.
+  assert (1 < length l).
+  apply leb_complete_conv. assumption.
+  split.
+  apply (le_lt_trans _ (div2 (length l))).
+  apply list_prefix_len. apply lt_div2.
+  transitivity 1; [ constructor | assumption ].
+  rewrite list_suffix_len.
+  apply lt_minus.
+  apply lt_le_weak. apply lt_div2.
+  transitivity 1; [ constructor | assumption ].
+  destruct l.
+  inversion H0.
+  destruct l.
+  inversion H0; inversion H2.
+  apply lt_0_Sn.
+Qed.
+
+Spec Definition decompose_smaller :
+  (forall l,
+     primitive l = false ->
+     smaller (fst (decompose l)) l /\ smaller (snd (decompose l)) l) :=
+  decompose_smallerH.
+
+
+(***
+ *** The compose operation, which requires list merge
+ ***)
+
+(* The length order on pairs of lists, which requires one of the two lists in
+the pair to be smaller and the other to be the same list; this is called the
+symmetric product of the length ordering. *)
+Definition list_pair_smaller : list nat * list nat -> list nat * list nat -> Prop :=
+  symprod _ _ smaller smaller.
+
+(* Merge two lists *)
 Function merge_lists (l_pair: list nat * list nat) {wf list_pair_smaller l_pair} : list nat :=
   let (l1,l2) := l_pair in
   match l1 with
@@ -135,20 +315,117 @@ Function merge_lists (l_pair: list nat * list nat) {wf list_pair_smaller l_pair}
             x2::merge_lists (l1,l2')
       end
   end.
-intros; apply plus_lt_compat_r; apply le_n.
-intros; apply plus_lt_compat_l; apply le_n.
-apply list_pair_smaller_wf.
+intros. apply left_sym. apply le_n.
+intros. apply right_sym. apply le_n.
+apply wf_symprod; apply smaller_wf.
 Defined.
+
+(* Helper lemma: merge_lists applied to two cons lists yields a result whose
+head is one of the two heads of the two lists. *)
+Lemma merge_lists_cons_cons x1 l1 x2 l2 :
+  {merge_lists (x1::l1, x2::l2) = x1::merge_lists (l1,x2::l2)} +
+  {merge_lists (x1::l1, x2::l2) = x2::merge_lists (x1::l1,l2)}.
+  assert (forall l_pair,
+            l_pair = (x1::l1, x2::l2) ->
+            {merge_lists l_pair = x1::merge_lists (l1,x2::l2)} +
+            {merge_lists l_pair = x2::merge_lists (x1::l1,l2)}).
+  intro l_pair; functional induction (merge_lists l_pair); intros; try discriminate.
+  injection H; intros.
+  rewrite H0; rewrite H1; rewrite H2; rewrite H3; left; reflexivity.
+  injection H; intros.
+  rewrite H0; rewrite H1; rewrite H2; rewrite H3; right; reflexivity.
+  apply H; reflexivity.
+Qed.
+
+(* Helper lemma: merging two sorted lists is sorted *)
+Lemma merge_lists_sorted l_pair :
+  sorted (fst l_pair) -> sorted (snd l_pair) -> sorted (merge_lists l_pair).
+  functional induction (merge_lists l_pair); unfold fst, snd; intros; try assumption.
+  unfold sorted; fold sorted.
+  destruct l1' as [ | x1' l1' ].
+  split.
+  apply lt_le_weak; assumption.
+  apply IHl; [ constructor | assumption ].
+  destruct (merge_lists_cons_cons x1' l1' x2 l2') as [ e_ml | e_ml ];
+    rewrite e_ml; rewrite <- e_ml.
+  split.
+  destruct H; assumption.
+  apply IHl; [ destruct H | ]; assumption.
+  split.
+  apply lt_le_weak; assumption.
+  apply IHl; [ destruct H | ]; assumption.
+  unfold sorted; fold sorted.
+  destruct l2' as [ | x2' l2' ].
+  split.
+  destruct (le_or_lt x2 x1); [ assumption | contradiction ].
+  assumption.
+  destruct (merge_lists_cons_cons x1 l1' x2' l2') as [ e_ml | e_ml ];
+    rewrite e_ml; rewrite <- e_ml.
+  split.
+  destruct (le_or_lt x2 x1); [ assumption | contradiction ].
+  apply IHl; [ assumption | destruct H0; assumption ].
+  split.
+  destruct H0; assumption.
+  apply IHl; [ assumption | destruct H0; assumption ].
+Qed.
+
+(* Helper lemma: merging lists yields a permutation of the original lists *)
+Lemma merge_lists_permOf l_pair :
+  permOf (fst l_pair ++ snd l_pair) (merge_lists l_pair).
+  functional induction (merge_lists l_pair); unfold fst, snd.
+  intro x; reflexivity.
+  intro x; rewrite app_nil_r; reflexivity.
+  apply permOf_cons; fold (app l1'); apply IHl.
+  apply (permOf_trans _ (x2 :: (x1 :: l1') ++ l2')).
+  apply permOf_app_cons.
+  apply permOf_cons. apply IHl.
+Qed.
 
 Spec Definition compose : (R -> R -> R) := (fun l1 l2 => merge_lists (l1,l2)).
 
-Spec Definition direct_solve : (D -> R) := (fun l => l).
 
-(* Soundness axioms *)
-Spec Axiom direct_solve_correct :
-  (forall d, primitive d = true -> IO d (direct_solve d)).
-Spec Axiom solve_soundness :
-  (forall d z1 z2,
-     IO (fst (decompose d)) z1 ->
-     IO (snd (decompose d)) z2 ->
-     IO d (compose z1 z2)).
+(***
+ *** Correctness theorems for the base and step cases
+ ***)
+
+(* Theorem: direct_solve is correct for primitive problems *)
+Spec Theorem direct_solve_correct :
+  (forall l, primitive l = true -> IO l (direct_solve l)).
+  unfold primitive, D, IO, direct_solve, def; intros.
+  destruct l.
+  (* Prove correctness for the empty list *)
+  split.
+  unfold sorted; trivial.
+  unfold permOf; intros; reflexivity.
+
+  destruct l.
+  (* Prove correctness for singleton lists *)
+  split.
+  unfold sorted; trivial.
+  unfold permOf; intros; reflexivity.
+
+  (* Lists with more than 1 element contradict primitive l = true *)
+  discriminate H.
+Qed.
+
+
+(* Theorem: if we solve the two decomposed problems then composing them is a
+solution *)
+Spec Theorem solve_soundness :
+  (forall l lout1 lout2,
+     IO (fst (decompose l)) lout1 ->
+     IO (snd (decompose l)) lout2 ->
+     IO l (compose lout1 lout2)).
+  unfold D, R, decompose, compose, IO, def, fst, snd.
+  intros l lout1 lout2 conj1 conj2; destruct conj1; destruct conj2.
+  split.
+  apply merge_lists_sorted; assumption.
+  rewrite <- (list_prefix_suffix_eq (div2 (length l)) l).
+  apply (permOf_trans _ (lout1 ++ lout2)).
+  apply permOf_app; assumption.
+  fold (fst (lout1,lout2)); fold (snd (lout1,lout2)).
+  apply merge_lists_permOf.
+Qed.
+
+Spec End MergeSort0
+.
